reorder function in Gallina that reorders a sep list based on an
order expressed as a list of nat priorities, and correctness
proof stating that if the length of the order matches the length
of the sep list, we have iff1 between the sep list and the reordered
sep list

bedrock2/src/bedrock2Examples/LiveVerif/swap.v
@@ -566,8 +566,166 @@ Set Ltac Backtrace.
 (* end move *)
 
 
+Require Import Coq.Sorting.Permutation Coq.Sorting.Sorting.
+
+Module FstNatOrder <: Orders.TotalLeBool.
+  Definition t: Type := nat * nat.
+  Definition leb: t -> t -> bool :=
+    fun '(x, _) '(y, _) => Nat.leb x y.
+  Theorem leb_total: forall a1 a2, leb a1 a2 = true \/ leb a2 a1 = true.
+  Proof.
+    unfold leb. intros [x _] [y _]. destr (x <=? y)%nat. 1: auto.
+    right. apply Nat.leb_le. unfold lt in E. eapply Nat.le_trans. 2: exact E.
+    do 2 constructor.
+  Qed.
+End FstNatOrder.
+
+Module FstNatSorting := Sort FstNatOrder.
+
+
 Load LiveVerif.
 Import SepLogPredsWithAddrLast.
+
+Lemma seps'_Permutation: forall (l1 l2: list (mem -> Prop)),
+    Permutation l1 l2 -> iff1 (seps' l1) (seps' l2).
+Proof.
+  induction 1.
+  - reflexivity.
+  - simpl. rewrite IHPermutation. reflexivity.
+  - simpl. cancel.
+  - etransitivity; eassumption.
+Qed.
+
+Lemma seps_Permutation: forall (l1 l2: list (mem -> Prop)),
+    Permutation l1 l2 -> iff1 (seps l1) (seps l2).
+Proof.
+  intros.
+  etransitivity. 2: eapply seps'_iff1_seps.
+  etransitivity. 2: eapply seps'_Permutation; exact H.
+  symmetry. eapply seps'_iff1_seps.
+Qed.
+
+Fixpoint zip_with_counter{A: Type}(l: list A)(start: nat): list (A * nat) :=
+  match l with
+  | nil => nil
+  | x :: xs => (x, start) :: zip_with_counter xs (S start)
+  end.
+
+Definition zip_with_index{A: Type}(l: list A): list (A * nat) := zip_with_counter l 0.
+
+Lemma snd_zip_with_counter: forall {A: Type} (l: list A) (start: nat),
+    List.map snd (zip_with_counter l start) = List.seq start (List.length l).
+Proof. induction l; simpl; intros. 1: reflexivity. f_equal. apply IHl. Qed.
+
+Lemma snd_zip_with_index: forall {A: Type} (l: list A),
+    List.map snd (zip_with_index l) = List.seq 0 (List.length l).
+Proof. intros. apply snd_zip_with_counter. Qed.
+
+Lemma List__map_nth_seq_self{A: Type}(d: A)(l: list A):
+  List.map (fun i => List.nth i l d) (List.seq 0 (List.length l)) = l.
+Proof.
+  induction l; cbn -[List.nth]. 1: reflexivity.
+  unfold List.nth at 1.
+  f_equal.
+  etransitivity. 2: exact IHl.
+  rewrite <- List.seq_shift.
+  rewrite List.map_map.
+  reflexivity.
+Qed.
+
+Definition apply_permutation_with_default(p: list nat){A: Type}(l: list A)(d: A): list A :=
+  List.map (fun i => List.nth i l d) p.
+
+Definition apply_permutation(p: list nat){A: Type}(l: list A): list A :=
+  match l with
+  | nil => nil
+  | cons d _ => apply_permutation_with_default p l d
+  end.
+
+Lemma apply_permutation_with_default_is_Permutation: forall (p: list nat) A (l: list A) d,
+    Permutation p (List.seq 0 (List.length l)) ->
+    Permutation l (apply_permutation_with_default p l d).
+Proof.
+  unfold apply_permutation_with_default. intros.
+  eapply Permutation_trans. 2: {
+    eapply Permutation_map.
+    eapply Permutation_sym.
+    exact H.
+  }
+  rewrite List__map_nth_seq_self.
+  apply Permutation_refl.
+Qed.
+
+Lemma apply_permutation_is_Permutation: forall (p: list nat) (A: Type) (l: list A),
+    Permutation p (List.seq 0 (List.length l)) ->
+    Permutation l (apply_permutation p l).
+Proof.
+  intros. unfold apply_permutation. destruct l.
+  - apply Permutation_refl.
+  - apply apply_permutation_with_default_is_Permutation. assumption.
+Qed.
+
+Definition order_to_permutation(order: list nat): list nat :=
+  List.map snd (FstNatSorting.sort (zip_with_index order)).
+
+Lemma order_to_permutation_is_Permutation(order: list nat):
+    Permutation (order_to_permutation order) (List.seq 0 (List.length order)).
+Proof.
+  unfold order_to_permutation.
+  eapply Permutation_trans. {
+    eapply Permutation_map.
+    eapply Permutation_sym.
+    eapply FstNatSorting.Permuted_sort.
+  }
+  rewrite snd_zip_with_index.
+  eapply Permutation_refl.
+Qed.
+
+(* `order` and `l` must have the same length.
+    The i-th element of `order` is the sort key of the i-th element of `l`.
+    Returns `l` sorted according to these sort keys. *)
+Definition reorder(order: list nat){A: Type}(l: list A): list A :=
+  apply_permutation (order_to_permutation order) l.
+
+Lemma reorder_is_iff1: forall (order: list nat) (l: list (mem -> Prop)),
+    List.length order = List.length l ->
+    iff1 (seps l) (seps (reorder order l)).
+Proof.
+  intros.
+  apply seps_Permutation.
+  unfold reorder.
+  apply apply_permutation_is_Permutation.
+  rewrite <- H.
+  apply order_to_permutation_is_Permutation.
+Qed.
+
+Lemma reordering_test: forall addr1 addr2 addr3 addr4 v1_old v1_new v2 v3 v4 R (m0 m1: mem),
+    seps [addr1 |-> scalar v1_old; addr2 |-> scalar v2; addr3 |-> scalar v3; R] m0 ->
+    (* value at addr1 was updated, addr2 was consumed, addr4 was added, and order was changed: *)
+    seps [R; addr3 |-> scalar v3; addr4 |-> scalar v4; addr1 |-> scalar v1_new] m1 ->
+    (* desired order: *)
+    seps [addr1 |-> scalar v1_new; addr3 |-> scalar v3; addr4 |-> scalar v4; R] m1.
+Proof.
+  intros. (* 0                        1                    2                    3
+  H  : seps [addr1 |-> scalar v1_old; addr2 |-> scalar v2; addr3 |-> scalar v3; R] m0
+  H0 : seps [R; addr3 |-> scalar v3; addr4 |-> scalar v4; addr1 |-> scalar v1_new] m1
+  order :=  [3; 2;                   2;                   0                      ] *)
+  pose [3%nat; 2%nat; 2%nat; 0%nat] as order.
+  eassert (@iff1 mem _ _) as E. {
+    etransitivity.
+    1: match goal with
+       | _: seps ?l m1 |- _ => eapply (reorder_is_iff1 order l)
+       end.
+    1: reflexivity.
+    cbv [reorder].
+    let r := eval vm_compute in (order_to_permutation order) in
+        change (order_to_permutation order) with r.
+    cbv [apply_permutation apply_permutation_with_default List.map List.nth].
+    reflexivity.
+  }
+  eapply E.
+  exact H0.
+Qed.
 
 (* TODO: write down postcondition only at end *)
 Definition swap_locals: {f: list string * list string * cmd &
@@ -635,6 +793,15 @@ Definition swap: {f: list string * list string * cmd &
     change ((seps [a_addr |-> scalar b; b_addr |-> scalar b; R]) m') in H.
     change ((seps [b_addr |-> scalar t; a_addr |-> scalar b; R]) m'0) in H0.
     (* Note: order of sep clauses was changed *)
+
+Undelimit Scope live_scope.
+Close Scope live_scope.
+
+  match goal with
+  | HOld: seps _ ?mOld, H: seps _ ?m |- wp_cmd _ _ _ ?m _ _ => idtac HOld H
+  end.
+
+idtac.
 
     ret (@nil string).
     subst. intuition solve[cbn[seps] in *; ecancel_assumption].
